merge VarSet and VarSet' and use SetLike instance instead + add functionality for working with VarSet

Strips/Basic.lean
@@ -292,4 +292,153 @@ lemma sub_progression_iff_sub_regression {n} {pt : PlanningTask n} {S S' A} :
     have : s ∈ Sᶜ := h1 hs_regr
     simp_all
 
-end STRIPS
+-- TODO : documentation
+/-! ## VarSet -/
+namespace VarSet
+
+lemma mem_iff {n i} {V : VarSet n} : i ∈ V ↔ V[i] := by
+  unfold SetLike.instMembership
+  simp only [SetLike.coe, Fin.getElem_fin, Set.mem_setOf_eq]
+
+instance {n} {i : Fin n} {V : VarSet n} : Decidable (i ∈ V) := by
+  rw [mem_iff]
+  infer_instance
+
+@[reducible]
+instance {n} : HasSubset (VarSet n) where
+  Subset V V' := ∀ i ∈ V, i ∈ V'
+
+@[simp]
+lemma mem_empty {n i} : i ∉ (∅ : VarSet n) := by
+  unfold instEmptyCollection
+  simp [mem_iff]
+
+instance {n} : Union (VarSet n) where
+  union V V' := V ||| V'
+
+@[simp]
+lemma mem_union {n} {V V' : VarSet n} {i} : i ∈ V ∪  V' ↔ i ∈ V ∨ i ∈ V' := by
+  unfold instUnion
+  simp [mem_iff]
+
+@[simp]
+lemma empty_union {n} {V : VarSet n} : ∅ ∪ V = V := by
+  simp only [SetLike.ext_iff, mem_union, mem_empty, false_or, implies_true]
+
+@[simp]
+lemma union_empty {n} {V : VarSet n} : V ∪ ∅ = V := by
+  simp only [SetLike.ext_iff, mem_union, mem_empty, or_false, implies_true]
+
+instance {n} : Inter (VarSet n) where
+  inter V V' := V &&& V'
+
+@[simp]
+lemma mem_inter {n} {V V' : VarSet n} {i} : i ∈ V ∩ V' ↔ i ∈ V ∧ i ∈ V' := by
+  unfold instInter
+  simp [mem_iff]
+
+@[simp]
+lemma empty_inter {n} {V : VarSet n} : ∅ ∩ V = ∅ := by
+  simp only [SetLike.ext_iff, mem_inter, mem_empty, false_and, implies_true]
+
+@[simp]
+lemma inter_eq_empty_iff {n} {V V' : VarSet n} : V ∩ V' = ∅ ↔ ∀ i ∈ V, i ∉ V' := by
+  simp only [SetLike.ext_iff, mem_inter, mem_empty, iff_false, not_and]
+
+@[simp]
+lemma mem_insert {n} {V : VarSet n} {i j} : j ∈ (V.insert i) ↔ j ∈ V ∨ j = i := by
+  simp [insert, mem_iff]
+  grind
+
+@[simp]
+lemma mem_ofList {n} {l : List (Fin n)} {i} : i ∈ (ofList l) ↔ i ∈ l := by
+  simp only [ofList]
+  induction l with
+  | nil => simp only [List.foldr_nil, mem_empty, List.not_mem_nil]
+  | cons j l ih =>
+    grind only [List.mem_cons, = List.foldr_cons, mem_insert]
+
+instance {n} : Compl (VarSet n) where
+  compl V := ~~~V
+
+@[simp]
+lemma mem_compl {n} {V : VarSet n} {i} : i ∈ Vᶜ ↔ i ∉ V := by
+  unfold instCompl
+  simp [mem_iff]
+
+instance {n} : SDiff (VarSet n) where
+  sdiff V V' := V &&& ~~~V'
+
+@[simp]
+lemma mem_diff {n} {V V' : VarSet n} {i} : i ∈ V \ V' ↔ i ∈ V ∧ i ∉ V' := by
+  unfold instSDiff
+  simp [mem_iff]
+
+def foldl {α n} (f : α → Fin n → α) (init : α) (V : VarSet n) : α :=
+  Fin.foldl n (fun a i ↦ if i ∈ V then f a i else a) init
+
+lemma foldl_cons {α n} {V : VarSet n} {f : Fin n → α} {a as} :
+    a ∈ V.foldl (fun a i ↦ f i :: a) as ↔ (∃ i ∈ V, a = f i) ∨ a ∈ as := by
+  simp only [foldl]
+  induction V using BitVec.cons_induction with
+  | nil => simp
+  | @cons n' b V ih =>
+    simp only [mem_iff, Fin.getElem_fin, Fin.foldl_succ_last, Fin.val_last,
+      Fin.val_castSucc] at *
+    have h1 : ∀ i : Fin n', i.val ≠ n' := by omega
+    split
+    · simp only [BitVec.getElem_cons, h1, ↓reduceDIte, List.mem_cons, ih]
+      constructor
+      · grind
+      · rw [← or_assoc]
+        apply Or.imp_left
+        rintro ⟨i, h2, rfl⟩
+        split at h2
+        · grind
+        · apply Or.inr
+          use ⟨i.val, by omega⟩
+          simp [h2]
+    · simp only [BitVec.getElem_cons, h1, ↓reduceDIte, ih]
+      constructor
+      · grind
+      · apply Or.imp_left
+        rintro ⟨i, h2, rfl⟩
+        split at h2
+        · grind
+        · use ⟨i.val, by omega⟩
+          simp [h2]
+
+-- TODO : can this be done more efficiently?
+def map {n m} (V : VarSet n) (f : Fin n → Fin m) : VarSet m :=
+  V.foldl (fun V' i ↦ V'.insert (f i)) ∅
+  -- Fin.foldl n (fun V' i ↦ if i ∈ V then V'.insert (f i) else V') empty
+
+lemma mem_map {n m} {V : VarSet n} {f : Fin n → Fin m} {i} :  i ∈ V.map f ↔ (∃ j ∈ V, i = f j) := by
+  simp only [map, foldl, insert]
+  induction V using BitVec.cons_induction with
+  | nil => simp
+  | @cons n' b V ih =>
+    simp only [mem_iff, Fin.getElem_fin, Fin.foldl_succ_last, Fin.val_last,
+      Fin.val_castSucc] at *
+    have h1 : ∀ i : Fin n', i.val ≠ n' := by omega
+    split
+    · simp only [BitVec.getElem_cons, h1, ↓reduceDIte, BitVec.getElem_or, BitVec.getElem_twoPow,
+      Bool.or_eq_true, ih, decide_eq_true_eq]
+      constructor
+      · grind
+      · rintro ⟨i, h2, rfl⟩
+        split at h2
+        · grind
+        · apply Or.inl
+          use ⟨i.val, by omega⟩
+          simp [h2]
+    · simp only [BitVec.getElem_cons, h1, ↓reduceDIte, ih]
+      constructor
+      · grind
+      · rintro ⟨i, h2, rfl⟩
+        split at h2
+        · grind
+        · use ⟨i.val, by omega⟩
+          simp [h2]
+
+end STRIPS.VarSet
